src/Spec/PointEncoding.v
@@ -23,20 +23,19 @@ Section PointEncoding.
       | Word.WS b _ w' => b
     end.
 
-  Definition point_enc (p : CompleteEdwardsCurve.point) : Word.word (S sz) := let '(x,y) := proj1_sig p in
+  Definition point_enc (p : E.point) : Word.word (S sz) := let '(x,y) := proj1_sig p in
     Word.WS (sign_bit x) (enc y).
 
   Program Definition point_dec_with_spec :
-    {point_dec : Word.word (S sz) -> option CompleteEdwardsCurve.point
+    {point_dec : Word.word (S sz) -> option E.point
                | forall w x, point_dec w = Some x -> (point_enc x = w)
                } := PointEncodingPre.point_dec.
    
   Definition point_dec := Eval hnf in (proj1_sig point_dec_with_spec).
 
-  Instance point_encoding : encoding of CompleteEdwardsCurve.point as (Word.word (S sz)) := {
+  Instance point_encoding : encoding of E.point as (Word.word (S sz)) := {
     enc := point_enc;
     dec := point_dec;
     encoding_valid := PointEncodingPre.point_encoding_valid
   }.
-
 End PointEncoding.
